[refactor] Make room for exercise 1.

ex1/lib/adt/tree/viz.py
@@ -1,0 +1,22 @@
+from adt.tree import Tree
+from os import linesep
+from tempfile import NamedTemporaryFile
+
+
+def dot_print(expr: Tree) -> None:
+    from graphviz import Source
+
+    temp = """digraph G{
+edge [dir=forward]
+
+"""
+    nodes = {id(n): (i, n) for (i, n) in enumerate(expr.nodes)}
+    edges = {(nodes[id(n)][0], nodes[id(s)][0]) for n in expr.nodes for s in n.subtrees}
+
+    def translate_backslash(x): return str(x).replace("\\", "\\\\")
+
+    nodes_string = linesep.join([f"{i[0]} [label=\"{translate_backslash(i[1].root)}\"]" for n, i in nodes.items()])
+    edges_string = linesep.join([f"{n} -> {s}" for (n, s) in edges])
+    tmp_file = NamedTemporaryFile(delete=False)
+    s = Source(temp + nodes_string + linesep + edges_string + linesep + "}", filename=tmp_file.name)
+    s.view(filename=tmp_file.name)
