lab2/extra/demo-even-odd.v
@@ -1,0 +1,20 @@
+Require Import Nat.
+
+Section EO.
+
+  Inductive even : nat -> Prop :=
+  | even_O : even 0
+  | even_S : forall n, odd n -> even (S n)
+  with odd : nat -> Prop :=
+     | odd_S : forall n, even n -> odd (S n).
+
+  Compute is_even 8.
+    
+  Fixpoint is_even n :=
+    match n with
+      0 => True
+    | S 0 => False
+    | S (S k) => is_even k
+    end.
+
+End EO.
